wip: more work, very wip

Rz/Algebra/PCA.lean
@@ -1,247 +1,147 @@
-/-
-# Partial Combinatory Algebras
--/
-import Rz.Data.Bwd
-import Rz.Syntax.Magma
-import Rz.Syntax.Subst
+import Mathlib.Init.Order.Defs
+import Mathlib.Tactic.NthRewrite
+import Mathlib.Tactic.Use
 
+import Rz.Syntax.Magma
+import Rz.Data.Bwd
 
 universe u v w
 variable {α β : Type u}
 
 /-!
-# Partial Applicative Structures
+## Partial Applicative Systems
 -/
 
-/-- Notation typeclass for Eval. -/
-class HasEval (α : Type u) where
-  /-- Big-step evaluation relation. -/
-  Eval : (ρ : Bwd α) → FreeMagma α → α → Prop
+class PAS (α : Type u) where
+  /-- `a₁ · a₂ ↝ a₃` denotes that applying a₁ to a₂ reduces to a₃. -/
+  Ap : α → α → α → Prop
+    /-- The application relation is functional. -/
+  ap_functional : {a₁ a₂ v₁ v₂ : α} → Ap a₁ a₂ v₁ → Ap a₁ a₂ v₂ → v₁ = v₂
 
-def HasEval.Undefined [HasEval α] (ρ : Bwd α) (e : FreeMagma α) : Prop := (a : α) → ¬ (HasEval.Eval ρ e a)
-def HasEval.Defined [HasEval α] (ρ : Bwd α) (e : FreeMagma α) : Prop := ∃ (a : α), HasEval.Eval ρ e a
-def HasEval.Refines [HasEval α] (ρ₁ ρ₂ : Bwd α) (e₁ e₂ : FreeMagma α) : Prop := (a : α) → HasEval.Eval ρ₂ e₂ a → HasEval.Eval ρ₁ e₁ a
-def HasEval.Equiv [HasEval α] (ρ₁ ρ₂ : Bwd α) (e₁ e₂ : FreeMagma α) : Prop := HasEval.Refines ρ₂ ρ₁ e₂ e₁ ∧ HasEval.Refines ρ₁ ρ₂ e₁ e₂
+/-- Extend the small-step relation to a big-step relation on `FreeMagma α`. -/
+def PAS.Eval [PAS α] : (ρ : Bwd α) → FreeMagma α → α → Prop
+  | ρ, .var i, v => ∃ h, ρ.get ⟨i, h⟩ = v
+  | _, .const a, v => a = v
+  | ρ, .ap e₁ e₂, v => ∃ v₁ v₂, Eval ρ e₁ v₁ ∧ Eval ρ e₂ v₂ ∧ PAS.Ap v₁ v₂ v
 
-syntax term " ⊢ " magma " ↑" : term
-syntax term " ⊢ " magma " ↓" : term
 syntax term " ⊢ " magma " ⇓ " term:40 : term
+macro_rules
+| `($ρ:term ⊢ $e:magma ⇓ $a:term) => `(PAS.Eval $ρ («magma» $e) $a)
+
+namespace PAS
+/-- `Undefined ρ e` denotes that an expression `e` diverges when evaluated in environment `ρ`. -/
+def Undefined [PAS α] (ρ : Bwd α) (e : FreeMagma α) : Prop := (a : α) → ¬ (ρ ⊢ e ⇓ a)
+/-- `Defined ρ e` denotes that an expression `e` diverges when evaluated in environment `ρ`. -/
+def Defined [PAS α] (ρ : Bwd α) (e : FreeMagma α) : Prop := ∃ (a : α), ρ ⊢ e ⇓ a
+/-- `Refines ρ e₁ e₂` denotes that an expression `e₂` is least as defined as `e₁`. -/
+def Refines [PAS α] (ρ₁ : Bwd α) (e₁ : FreeMagma α) (ρ₂ : Bwd α) (e₂ : FreeMagma α) : Prop := {a : α} → ρ₁ ⊢ e₁ ⇓ a → ρ₂ ⊢ e₂ ⇓ a
+end PAS
+
+@[inherit_doc PAS.Undefined]
+syntax term " ⊢ " magma " ↑" : term
+@[inherit_doc PAS.Defined]
+syntax term " ⊢ " magma " ↓" : term
+@[inherit_doc PAS.Refines]
 syntax term " ⊢ " magma " ≤ " term:max " ⊢ " withPosition(magma) : term
-syntax term " ⊢ " magma " ≃ " term:max " ⊢ " withPosition(magma) : term
 
 macro_rules
-| `($ρ:term ⊢ $e:magma ↑) => `(HasEval.Undefined $ρ («magma» $e))
-| `($ρ:term ⊢ $e:magma ↓) => `(HasEval.Defined $ρ («magma» $e))
-| `($ρ:term ⊢ $e:magma ⇓ $a:term) => `(HasEval.Eval $ρ («magma» $e) $a)
-| `($ρ₁:term ⊢ $e₁:magma ≤ $ρ₂:term ⊢ $e₂:magma) => `(HasEval.Refines $ρ₂ $ρ₁ («magma» $e₂) («magma» $e₁))
-| `($ρ₁:term ⊢ $e₁:magma ≃ $ρ₂:term ⊢ $e₂:magma) => `(HasEval.Equiv $ρ₁ $ρ₂ («magma» $e₁) («magma» $e₂))
+| `($ρ:term ⊢ $e:magma ↑) => `(PAS.Undefined $ρ («magma» $e))
+| `($ρ:term ⊢ $e:magma ↓) => `(PAS.Defined $ρ («magma» $e))
+| `($ρ₁:term ⊢ $e₁:magma ≤ $ρ₂:term ⊢ $e₂:magma) => `(PAS.Refines $ρ₁ («magma» $e₁) $ρ₂ («magma» $e₂))
 
-/-- Partial Applicative Structures. -/
-class PAS (α : Type u) extends HasEval α where
-  /-- The evaluation relation is functional. -/
-  eval_functional : {ρ : Bwd α} → {e : FreeMagma α} → {a a' : α} → ρ ⊢ e ⇓ a → ρ ⊢ e ⇓ a' → a = a'
-  /-- Looking up the 0th variable resolves to the final element of the environment. -/
-  var_zero_eval : (ρ : Bwd α) → (a : α) → (ρ :# a) ⊢ `(0) ⇓ a
-  /-- Resolving a successor variable requires us to look up in the tail of the environment. -/
-  var_succ_eval_le : (ρ : Bwd α) → (a : α) → (n : Nat) → (ρ :# a) ⊢ `(n+1) ≤ ρ ⊢ `(n)
-  var_succ_eval_ge : (ρ : Bwd α) → (a : α) → (n : Nat) → ρ ⊢ `(n) ≤ (ρ :# a) ⊢ `(n+1)
-  /-- Resolving an out-of-bounds variable diverges. -/
-  var_zero_diverge : (n : Nat) → (Bwd.nil : Bwd α) ⊢ `(n) ↑
-  /-- Constants reduce to themselves. -/
-  const_eval : (ρ : Bwd α) → (a : α) → ρ ⊢ a ⇓ a
-  /-- Applications are evaluated by evaluating both sides.
-      Note the change of environment; this corresponds to the fact that substitutions do not act on values. -/
-  ap_eval_le : {ρ₁ ρ₂ : Bwd α} → {e₁ e₂ : FreeMagma α} → {a₁ a₂ : α} → ρ₁ ⊢ e₁ ⇓ a₁ → ρ₁ ⊢ e₂ ⇓ a₂ → ρ₁ ⊢ e₁ e₂ ≤ ρ₂ ⊢ a₁ a₂
-  ap_eval_ge : {ρ₁ ρ₂ : Bwd α} → {e₁ e₂ : FreeMagma α} → {a₁ a₂ : α} → ρ₁ ⊢ e₁ ⇓ a₁ → ρ₁ ⊢ e₂ ⇓ a₂ → ρ₂ ⊢ a₁ a₂ ≤ ρ₁ ⊢ e₁ e₂
-  /-- If an application is defined, then so is the left argument. -/
-  ap_left_defined : {ρ : Bwd α} → {e₁ e₂ : FreeMagma α} → ρ ⊢ e₁ e₂ ↓ → ρ ⊢ e₁ ↓
-  /-- If an application is defined, then so is the right argument. -/
-  ap_right_defined : {ρ : Bwd α} → {e₁ e₂ : FreeMagma α} → ρ ⊢ e₁ e₂ ↓ → ρ ⊢ e₂ ↓
 
 namespace PAS
 
 /-!
-## Variable Lemmas
+### Order-Theoretic Properties of Refinement
 -/
 
-/-- Variant of `var_succ_eval` that uses `Nat.pred`. -/
-theorem var_pred_eval_ne_zero_le
-  [PAS α]
-  (ρ : Bwd α) (a : α)
-  (n : Nat) (h : n ≠ 0)
-  : (ρ :# a) ⊢ `(n) ≤ ρ ⊢ `(n.pred) := by
-  match n with
-  | 0 => contradiction
-  | n+1 => apply var_succ_eval_le
+/-- The refinement relation extends to a preorder on expressions. -/
+instance Refine [PAS α] {ρ : Bwd α} : Preorder (FreeMagma α) where
+  le e₁ e₂ := PAS.Refines ρ e₁ ρ e₂
+  le_refl e v v_eval := v_eval
+  le_trans e₁ e₂ e₃ p q v v_eval := q (p v_eval)
+variable [PAS α]
 
-theorem var_pred_eval_ne_zero_ge
-  [PAS α]
-  (ρ : Bwd α) (a : α)
-  (n : Nat) (h : n ≠ 0)
-  : ρ ⊢ `(n.pred) ≤ (ρ :# a) ⊢ `(n) := by
-  match n with
-  | 0 => contradiction
-  | n+1 => apply var_succ_eval_ge
-
-
-/-- Variable lookups evaluate to `Bwd.get` if they are in bounds. -/
-theorem var_get_eval
-  [PAS α]
-  (ρ : Bwd α) (x : Fin ρ.length)
-  : ρ ⊢ `(x) ⇓ ρ.get x := by
-  match ρ with
-  | .nil =>
-    have : x.val < 0 := x.is_lt
-    contradiction
-  | .snoc ρ a =>
-    if h : x = 0 then
-      simp [h]
-      apply PAS.var_zero_eval
-    else
-      apply (PAS.var_pred_eval_ne_zero_ge ρ a x (Fin.val_ne_of_ne h))
-      rw [Bwd.get_snoc_pred_ne_zero ρ a x h]
-      apply PAS.var_get_eval (x := x.pred h)
-
-theorem var_of_converge [PAS α] (ρ : Bwd α) (x : Nat) : ρ ⊢ `(x) ↓ → x < ρ.length := by
-  rintro ⟨v, H⟩
-  induction ρ generalizing x with
-  | nil => cases var_zero_diverge _ _ H
-  | snoc ρ a IH =>
-    match x with
-    | 0 => simp
-    | x + 1 => exact Nat.succ_lt_succ <| IH _ <| var_succ_eval_le _ _ _ _ H
-
-/-!
-## Evaluation Lemmas
--/
-
-/-- If a value evaluates to another value, then the two values are equal. -/
-theorem const_eval_eq
-  [PAS α]
-  (ρ : Bwd α)
-  (a a' : α) (a_eval : ρ ⊢ a ⇓ a')
-  : a = a' :=
-    eval_functional (const_eval ρ a) a_eval
-
-
-/-- Evaluation of constants is invariant under environments. -/
-theorem const_eval_stable
-  [PAS α]
-  (ρ₁ ρ₂ : Bwd α)
-  (a a' : α) (a_eval : ρ₁ ⊢ a ⇓ a')
-  : ρ₂ ⊢ a ⇓ a' := by
-    rw [const_eval_eq ρ₁ a a' a_eval]
-    apply const_eval
-
-/-- Evaluation of closed terms is invariant under environments. -/
-theorem closed_eval_stable
-  [PAS α]
-  (ρ₁ ρ₂ : Bwd α)
-  (e : FreeMagma α) (a : α)
-  (closed : e.fv = 0)
-  (a_eval : ρ₁ ⊢ e ⇓ a)
-  : ρ₂ ⊢ e ⇓ a := by
-    match e with
-    | .var _ => contradiction
-    | .const b =>
-       apply const_eval_stable
-       exact a_eval
-    | .ap e₁ e₂ =>
-      have ⟨ a₁ , a₁_eval_ρ₁ ⟩ := ap_left_defined ⟨ a , a_eval ⟩
-      have ⟨ a₂ , a₂_eval_ρ₁ ⟩ := ap_right_defined ⟨ a , a_eval ⟩
-      have ⟨ e₁_closed , e₂_closed ⟩ := FreeMagma.ap_closed_closed closed
-      have a₁_eval_ρ₂ : ρ₂ ⊢ e₁ ⇓ a₁ := by
-        apply closed_eval_stable
-        · exact e₁_closed
-        · exact a₁_eval_ρ₁
-      have a₂_eval_ρ₂ : ρ₂ ⊢ e₂ ⇓ a₂ := by
-        apply closed_eval_stable
-        · exact e₂_closed
-        · exact a₂_eval_ρ₁
-      apply ap_eval_ge a₁_eval_ρ₂ a₂_eval_ρ₂
-      apply ap_eval_le (ρ₂ := ρ₂) a₁_eval_ρ₁ a₂_eval_ρ₁
-      · exact a_eval
-
-/-!
-## Definedness Lemmas
--/
-
-/-- Constants are always defined. -/
-theorem const_defined [PAS α] (ρ : Bwd α) (a : α) : ρ ⊢ a ↓ :=
-  ⟨ a , const_eval ρ a ⟩
-
-/-- An application is defined when both sides evalute to a value, and the application of those values is defined. -/
-theorem ap_defined
-  [PAS α]
-  {ρ : Bwd α} {e₁ e₂ : FreeMagma α} {a₁ a₂ : α}
-  (e₁_def : ρ ⊢ e₁ ⇓ a₁) (e₂_def : ρ ⊢ e₂ ⇓ a₂)
-  (v_def : ρ ⊢ a₁ a₂ ↓)
-  : ρ ⊢ e₁ e₂ ↓ :=
-    let ⟨ w , h ⟩ := v_def
-    ⟨ w , ap_eval_ge e₁_def e₂_def w h ⟩
-
-def refine_refl
-  [PAS α]
-  {ρ : Bwd α} {e : FreeMagma α}
-  : ρ ⊢ e ≤ ρ ⊢ e := by
-  intros _ v_eval
-  exact v_eval
-
-def ap_refine
-  [PAS α]
-  {ρ : Bwd α} {e₁ e₂ e₁' e₂' : FreeMagma α}
-  (rl : ρ ⊢ e₁ ≤ ρ ⊢ e₁')
-  (rr : ρ ⊢ e₂ ≤ ρ ⊢ e₂')
+/-- Application is monotonic with respect to refinement. -/
+theorem ap_le_ap
+  {ρ : Bwd α}
+  {e₁ e₂ e₁' e₂' : FreeMagma α}
+  (le_left : ρ ⊢ e₁ ≤ ρ ⊢ e₁') (le_right : ρ ⊢ e₂ ≤ ρ ⊢ e₂')
   : ρ ⊢ e₁ e₂ ≤ ρ ⊢ e₁' e₂' := by
-  intros v v_eval
-  have ⟨ v₁ , v₁_eval ⟩ := ap_left_defined ⟨ v , v_eval ⟩
-  have ⟨ v₂ , v₂_eval ⟩ := ap_right_defined ⟨ v , v_eval ⟩
-  apply ap_eval_ge
-  · exact rl v₁ v₁_eval
-  · exact rr v₂ v₂_eval
-  · apply ap_eval_le (ρ₂ := ρ)
-    · exact v₁_eval
-    · exact v₂_eval
-    · exact v_eval
+    intros v v_eval
+    simp [Eval] at *
+    have ⟨ v₁ , v₁_eval , v₂ , v₂_eval, v_ap ⟩ := v_eval
+    exact ⟨ v₁ , le_left v₁_eval, v₂ , le_right v₂_eval, v_ap ⟩
 
-def ap_refine_left
-  [PAS α]
-  {ρ : Bwd α} {e₁ e₂ e₁' : FreeMagma α}
-  (h : ρ ⊢ e₁ ≤ ρ ⊢ e₁')
-  : ρ ⊢ e₁ e₂ ≤ ρ ⊢ e₁' e₂ :=
-  ap_refine h refine_refl
+@[inherit_doc ap_le_ap]
+theorem ap_le_ap_right
+  {ρ : Bwd α}
+  {e₁ e₂ e₂' : FreeMagma α}
+  (le_right : ρ ⊢ e₂ ≤ ρ ⊢ e₂')
+  : ρ ⊢ e₁ e₂ ≤ ρ ⊢ e₁ e₂' := ap_le_ap (Refine.le_refl e₁) le_right
 
-def ap_refine_right
-  [PAS α]
-  {ρ : Bwd α} {e₁ e₂ e₂' : FreeMagma α}
-  (h : ρ ⊢ e₂ ≤ ρ ⊢ e₂')
-  : ρ ⊢ e₁ e₂ ≤ ρ ⊢ e₁ e₂' :=
-  ap_refine refine_refl h
+@[inherit_doc ap_le_ap]
+theorem ap_le_ap_left
+  {ρ : Bwd α}
+  {e₁ e₂ e₁' : FreeMagma α}
+  (le_left : ρ ⊢ e₁ ≤ ρ ⊢ e₁')
+  : ρ ⊢ e₁ e₂ ≤ ρ ⊢ e₁' e₂ := ap_le_ap le_left (Refine.le_refl e₂)
 
-def ap_congl
-  [PAS α]
-  {ρ : Bwd α} {e₁ e₂ : FreeMagma α} {v₁ : α}
-  (e₁_eval : ρ ⊢ e₁ ⇓ v₁)
-  : ρ ⊢ e₁ e₂ ≤ ρ ⊢ v₁ e₂ := by
-  apply ap_refine_left
-  intros v v_eval
-  have : v = v₁ := eval_functional v_eval e₁_eval
-  rw [this]
-  apply const_eval
+theorem ap_eval
+  {ρ : Bwd α}
+  {e₁ e₂ : FreeMagma α} {v : α}
+  : ρ ⊢ e₁ e₂ ⇓ v ↔ ∃ v₁ v₂ : α, ρ ⊢ e₁ ⇓ v₁ ∧  ρ ⊢ e₂ ⇓ v₂ ∧ PAS.Ap v₁ v₂ v := by simp [PAS.Eval]
 
-def ap_congr
-  [PAS α]
-  {ρ : Bwd α} {e₁ e₂ : FreeMagma α} {v₂ : α}
-  (e₂_eval : ρ ⊢ e₂ ⇓ v₂)
-  : ρ ⊢ e₁ e₂ ≤ ρ ⊢ e₁ v₂ := by
-  apply ap_refine_right
-  intros v v_eval
-  have : v = v₂ := eval_functional v_eval e₂_eval
-  rw [this]
-  apply const_eval
+theorem ap_congl
+  {ρ : Bwd α}
+  {e₁ e₂ : FreeMagma α} {v : α}
+  : ρ ⊢ e₁ e₂ ⇓ v ↔ ∃ v₁ : α, ρ ⊢ e₁ ⇓ v₁ ∧ ρ ⊢ v₁ e₂ ⇓ v := by
+  simp [PAS.Eval]
+
+theorem ap_congr
+  {ρ : Bwd α}
+  {e₁ e₂ : FreeMagma α} {v : α}
+  : ρ ⊢ e₁ e₂ ⇓ v ↔ ∃ v₂ : α, ρ ⊢ e₂ ⇓ v₂ ∧ ρ ⊢ e₁ v₂ ⇓ v := by
+  simp [PAS.Eval]
+  apply Iff.intro
+  · rintro ⟨ v₁ , v₁_eval , v₂ , v₂_eval , v_ap ⟩
+    exact ⟨ v₂ , v₂_eval , v₁ , v₁_eval , v_ap ⟩
+  · rintro ⟨ v₂ , v₂_eval , v₁ , v₁_eval , v_ap ⟩
+    exact ⟨ v₁ , v₁_eval , v₂ , v₂_eval , v_ap ⟩
+
+@[simp] theorem const_eval
+  {ρ : Bwd α}
+  {a v : α}
+  : ρ ⊢ a ⇓ v ↔ a = v := by
+  simp [PAS.Eval]
+
+/-!
+### Evaluation Lemmas
+-/
+
+/-- Evaluation is a functional relation. -/
+theorem eval_functional
+    {ρ : Bwd α}
+    {e : FreeMagma α} {a a' : α}
+    (h1 : ρ ⊢ e ⇓ a) (h2 : ρ ⊢ e ⇓ a')
+    : a = a' := by
+  induction e generalizing a a' with simp [Eval] at h1 h2
+  | var => obtain ⟨_, rfl⟩ := h1; obtain ⟨_, rfl⟩ := h2; rfl
+  | const => exact h1 ▸ h2
+  | ap _ _ ih1 ih2 =>
+    obtain ⟨_, ev11, _, ev12, h1⟩ := h1
+    obtain ⟨_, ev21, _, ev22, h2⟩ := h2
+    cases ih1 ev11 ev21
+    cases ih2 ev12 ev22
+    exact ap_functional h1 h2
 
 
 end PAS
+
+/-!
+# Partial Combinatory Algebras
+-/
 
 /-- Partial Combinatory Algebras. -/
 class PCA (α : Type u) extends PAS α where
@@ -250,179 +150,125 @@ class PCA (α : Type u) extends PAS α where
   /-- Bracket abstraction yields a value. -/
   abs_defined : (ρ : Bwd α) → (e : FreeMagma α) → ρ ⊢ $(abs e) ↓
   /-- Bracket abstraction has a β-law. -/
-  abs_eval_le : (ρ : Bwd α) → (a : α) → (e : FreeMagma α) → ρ ⊢ $(abs e) a ≤ (ρ :# a) ⊢ e
-  abs_eval_ge : (ρ : Bwd α) → (a : α) → (e : FreeMagma α) → (ρ :# a) ⊢ e ≤ ρ ⊢ $(abs e) a
+  abs_eval : {ρ : Bwd α} → {e₁ e₂ : FreeMagma α} → {v₁ : α} → ρ ⊢ $(abs e₁) e₂ ⇓ v₁ ↔ (∃ v₂, ρ ⊢ e₂ ⇓ v₂ ∧ (ρ :# v₂) ⊢ e₁ ⇓ v₁)
 
 namespace PCA
 
-protected def i [PCA α] : FreeMagma α :=
+variable [PCA α]
+
+def absn (e : FreeMagma α) (n : Nat) : FreeMagma α :=
+  match n with
+  | 0 => e
+  | n+1 => (absn (abs e) n)
+
+theorem absn_le
+  {ρ : Bwd α} {e : FreeMagma α} {as : Bwd (FreeMagma α)} {v : α} {vargs : Bwd α}
+  (e_eval : ρ ⊢ $(absn e as.length) $[as]* ⇓ v)
+  (h : as.length = vargs.length)
+  (as_eval : ∀ (i : Fin as.length), ρ ⊢ $(as.get i) ⇓ vargs.get (Fin.cast h i))
+  : (ρ ++ vargs) ⊢ e ⇓ v := by
+    match as, vargs with
+    | .nil, .nil =>
+      simp [absn] at *
+      exact e_eval
+    | .snoc as a, .snoc vargs varg =>
+      simp [absn, Bwd.foldBwd_snoc] at *
+      have ⟨ vbody , vbody_eval , v_ap ⟩ := PAS.ap_congl.1 e_eval
+      have ih_eval := absn_le (vargs := vargs) vbody_eval sorry sorry
+      have a_eval := as_eval 0
+      simp at a_eval
+      have outer_eval : (ρ ++ vargs) ⊢ $(abs e) varg ⇓ v := by
+        rw [PAS.ap_congl]
+        use _, ih_eval
+        sorry
+        -- simp [PAS.Eval]
+        -- sorry
+      have ⟨ varg', varg_eq, final_eval ⟩ := abs_eval.1 outer_eval
+      simp at varg_eq
+      rwa [varg_eq]
+
+protected def id : FreeMagma α :=
   abs (.var 0)
 
-protected def i_eval_le [PCA α] (ρ : Bwd α) (e : FreeMagma α) : ρ ⊢ PCA.i e ≤ ρ ⊢ e := by
-  intros v v_eval
-  have ⟨ v' , v'_eval ⟩ := PAS.ap_right_defined ⟨ v , v_eval ⟩
-  have : ρ ⊢ PCA.i v' ⇓ v := PAS.ap_congr v'_eval _ v_eval
-  have l : (ρ :# v') ⊢ `(0) ⇓ v := abs_eval_le ρ v' (.var 0) v this
-  have r : (ρ :# v') ⊢ `(0) ⇓ v' := by
-   apply PAS.var_zero_eval
-  have : v = v' := PAS.eval_functional l r
-  rwa [this]
+protected theorem id_le (ρ : Bwd α) (e : FreeMagma α) : ρ ⊢ PCA.id e ≤ ρ ⊢ e := by
+  intro v v_eval
+  rewrite [PCA.id, PCA.abs_eval] at v_eval
+  simp [PAS.Eval] at v_eval
+  exact v_eval
 
-protected def i_eval_ge [PCA α] (ρ : Bwd α) (e : FreeMagma α) : ρ ⊢ e ≤ ρ ⊢ PCA.i e := by
-  intros v v_eval
-  have : ρ ⊢ PCA.i v ⇓ v := by
-    apply abs_eval_ge ρ v (.var 0)
-    apply PAS.var_zero_eval
-  exact (PAS.ap_congr_inv this v_eval)
+protected theorem le_id (ρ : Bwd α) (e : FreeMagma α) : ρ ⊢ e ≤ ρ ⊢ PCA.id e := by
+  intro v v_eval
+  simp [PCA.id, PCA.abs_eval]
+  simp [PAS.Eval]
+  exact v_eval
 
-protected def i_eval_eq
-  [PCA α] {ρ : Bwd α} {v v' : α}
-  (v_eval : ρ ⊢ PCA.i v ⇓ v')
-  : v = v' := by
-    apply PAS.eval_functional (ρ := ρ)
-    · apply PCA.i_eval_ge
-      · apply PAS.const_eval
-    · exact v_eval
+@[simp] protected theorem i_eval {ρ : Bwd α} {e : FreeMagma α} {v : α} : ρ ⊢ PCA.id e ⇓ v ↔ ρ ⊢ e ⇓ v :=
+  ⟨ PCA.id_le _ _ , PCA.le_id _ _ ⟩
 
-protected def c [PCA α] (e₁ e₂ : FreeMagma α) : FreeMagma α :=
-  abs («magma» e₂ (e₁ `(0)))
+-- \f g x.
+protected def comp : FreeMagma α :=
+  abs (abs (abs («magma» `(1) (`(2) `(0)))))
 
--- protected def c_eval_le
---   [PCA α]
---   {ρ : Bwd α}
---   {e₁ e₂ : FreeMagma α} {v₁ v₂ : α}
---   (e₁_eval : ρ ⊢ e₁ ⇓ v₁) (e₂)
+protected theorem comp_le
+  {ρ : Bwd α} {e₁ e₂ e₃ : FreeMagma α} {v : α}
+  : ρ ⊢ PCA.comp e₁ e₂ e₃ ≤ ρ ⊢ e₂ (e₁ e₃) := by
+  intro v v_eval
+  sorry
 
-protected def true [PCA α] : FreeMagma α :=
-  (abs (abs (.var 1)))
+protected theorem le_comp
+  {ρ : Bwd α} {e₁ e₂ e₃ : FreeMagma α} {v : α}
+  : ρ ⊢ e₂ (e₁ e₃) ≤ ρ ⊢ PCA.comp e₁ e₂ e₃ :=
+  sorry
 
-protected def false [PCA α] : FreeMagma α :=
-  (abs (abs (.var 0)))
 
-protected def ite [PCA α] : FreeMagma α :=
-  (abs (abs (abs («magma» `(2) `(1) `(0)))))
+@[simp] protected theorem comp_eval
+  {ρ : Bwd α} {e₁ e₂ e₃ : FreeMagma α} {v : α}
+  : ρ ⊢ PCA.comp e₁ e₂ e₃ ⇓ v ↔ ρ ⊢ e₂ (e₁ e₃) ⇓ v :=
+  ⟨ PCA.comp_le (v := v) , PCA.le_comp (v := v) ⟩
+-- @[simp] protected def comp_eval {ρ : Bwd α} {e₁ e₂ e₃ : FreeMagma α} {v : α} : ρ ⊢ PCA.comp e ⇓ v ↔ ρ ⊢ e ⇓ v := sorry
+
+-- protected def le_comp (ρ : Bwd α) (e₁ e₂ e₃ : FreeMagma α) : ρ ⊢ e₂ (e₁ e₃) ≤ ρ ⊢ PCA.comp e₁ e₂ e₃ := by
+--   apply PAS.ap_le_ap_var_right
+--   sorry
+  -- rintro v ⟨ v₂ , v₁₃ , v₂_eval , ⟨ v₁ , v₃ , v₁_eval , v₂_eval , v₁₃_ap ⟩ , v_ap ⟩
+  -- suffices h : (ρ :# v₃ :# v₂ :# v₁) ⊢ PCA.comp `(0) `(1) `(2) ⇓ v
+  -- · sorry
+  -- · sorry
+  -- have
+  -- apply PAS.ap_le_ap_left
+  -- · apply PAS.ap_le_ap_left
+  --   · unfold PCA.comp
+  --     sorry
+  --   · sorry
+  -- · sorry
+  -- rw [PAS.ap_congl]
+  -- exists sorry
+  -- rw [PAS.ap_congl]
+  -- exists sorry
+  -- rintro v ⟨ v₂ , v₁ , v₂_eval , ⟨ v₁ , v₃ , p ⟩ , v_ap ⟩
+  -- rw [PCA.comp, PAS.ap_eval]
+  -- exists sorry
+  -- exists v
+  -- rw [PAS.ap_eval]
+  -- split_ands
+  -- · exists sorry
+  --   exists sorry
+  --   rw [PCA.abs_eval]
+  --   sorry
+  -- · sorry
+  -- · sorry
+  -- exists sorry
+  -- rw [PCA.abs_eval]
+  -- exact ⟨ sorry , sorry , sorry ⟩
+
+-- protected def comp_le (ρ : Bwd α) (e₁ e₂ e₃ : FreeMagma α) : ρ ⊢ PCA.comp e₁ e₂ e₃ ≤ ρ ⊢ e₂ (e₁ e₃) := by
+--   intros v v_eval
+--   rewrite [PCA.comp] at v_eval
+--   sorry
+--   -- have ⟨ v_comp , v_comp_eval ⟩ := abs_defined ρ (.ap e₂ (.ap e₁ (.var 0)))
+--   -- have ⟨ v₂ , v₂_eval , v' , ⟨ v₁ , v₁_eval , v₃ , v₃_eval , v'_ap ⟩ , v_ap ⟩ := v_eval
+--   -- have ⟨ v₁ , v₂ , v₁_eval , v_v₂_eq, v_ap ⟩ : ρ ⊢ $(abs (.var 0)) v ⇓ v :=
+--   --   abs_eval ρ v (FreeMagma.var 0)  (by simp [PAS.Eval])
+--   -- exact ⟨ v_comp , v_comp_eval , v₃, v₃_eval, sorry ⟩
 
 end PCA
-
-/-!
-# SKI forms a basis for PCAs (and v.v.)
--/
-
-/-- Partial Applicative Structures with S, K, and I combinators. -/
-class SKI (α : Type u) extends PAS α where
-  s : α
-  k : α
-  i : α
-  s_defined_2 : {ρ : Bwd α} → {e₁ e₂ : FreeMagma α} → ρ ⊢ e₁ ↓ → ρ ⊢ e₂ ↓ → ρ ⊢ s e₁ e₂ ↓
-  k_defined : {ρ : Bwd α} → {e : FreeMagma α} → ρ ⊢ e ↓ → ρ ⊢ k e ↓
-  s_eval_le : (ρ : Bwd α) → (e₁ e₂ e₃ : FreeMagma α) → ρ ⊢ s e₁ e₂ e₃ ≤ ρ ⊢ (e₁ e₃) (e₂ e₃)
-  s_eval_ge : (ρ : Bwd α) → (e₁ e₂ e₃ : FreeMagma α) → ρ ⊢ (e₁ e₃) (e₂ e₃) ≤ ρ ⊢ s e₁ e₂ e₃
-  k_eval_le : (ρ : Bwd α) → (e₁ e₂ : FreeMagma α) → ρ ⊢ e₂ ↓ → ρ ⊢ k e₁ e₂ ≤ ρ ⊢ e₁
-  k_eval_ge : (ρ : Bwd α) → (e₁ e₂ : FreeMagma α) → ρ ⊢ e₂ ↓ → ρ ⊢ e₁ ≤ ρ ⊢ k e₁ e₂
-  i_eval_le : (ρ : Bwd α) → (e : FreeMagma α) → ρ ⊢ i e ≤ ρ ⊢ e
-  i_eval_ge : (ρ : Bwd α) → (e : FreeMagma α) → ρ ⊢ e ≤ ρ ⊢ i e
-
-namespace SKI
-
-open SKI
-
-theorem s_defined_1
-  [A : SKI α]
-  {ρ : Bwd α} {e : FreeMagma α}
-  (e_defined : ρ ⊢ e ↓)
-  : ρ ⊢ A.s e ↓ :=
-  PAS.ap_left_defined (s_defined_2 e_defined (PAS.const_defined ρ k))
-
-@[simp] def abs [SKI α] : FreeMagma α → FreeMagma α
-| .var 0 => .const i
-| .var (n+1) => .ap (.const k) (.var n)
-| .const a => .ap (.const k) (.const a)
-| .ap e₁ e₂ => .ap (.ap (.const s) (abs e₁)) (abs e₂)
-
-def abs_defined [SKI α] (ρ : Bwd α) (e : FreeMagma α) (h : e.fv ≤ ρ.length + 1) : ρ ⊢ $(SKI.abs e) ↓ := by
-  match e with
-  | .var 0 => simp; apply PAS.const_defined
-  | .var (n+1) =>
-    simp
-    apply PAS.ap_defined
-    · apply PAS.const_eval
-    · apply PAS.var_get_eval ρ ⟨ n , Nat.le_of_succ_le_succ h ⟩
-    · apply SKI.k_defined
-      apply PAS.const_defined
-  | .const a =>
-    simp
-    apply PAS.ap_defined
-    · apply PAS.const_eval
-    · apply PAS.const_eval
-    · apply SKI.k_defined
-      apply PAS.const_defined
-  | .ap e₁ e₂ =>
-    simp
-    apply s_defined_2
-    · have : e₁.fv ≤ ρ.length + 1 := Trans.trans (FreeMagma.fv_left_le_fv_ap e₁ e₂) h
-      exact SKI.abs_defined ρ e₁ this
-    · have : e₂.fv ≤ ρ.length + 1 := Trans.trans (FreeMagma.fv_right_le_fv_ap e₁ e₂) h
-      exact SKI.abs_defined ρ e₂ this
-
-def abs_refines_le [SKI α] (ρ : Bwd α) (a : α) (e : FreeMagma α) : ρ ⊢ $(abs e) a ≤ (ρ :# a) ⊢ e := by
-  intros v v_eval
-  match e with
-  | .var 0 =>
-    simp at *
-    have var_eval : (ρ :# a) ⊢ `(0) ⇓ a := PAS.var_zero_eval ρ a
-    have a_eval : ρ ⊢ a ⇓ v := i_eval_le _ _ v v_eval
-    rwa [←PAS.const_eval_eq ρ a v a_eval]
-  | .var (n+1) =>
-     simp at *
-     apply PAS.var_succ_eval_ge ρ a n
-     apply SKI.k_eval_le ρ (.var n) (.const a) _
-     · exact v_eval
-     · apply PAS.const_defined
-  | .const b =>
-    simp at *
-    apply PAS.const_eval_stable
-    apply SKI.k_eval_le ρ (.const b) (.const a) _
-    · exact v_eval
-    · apply PAS.const_defined ρ a
-  | .ap e₁ e₂ =>
-    simp at *
-    have ap_abs_eval : ρ ⊢ ($(abs e₁) a) ($(abs e₂) a) ⇓ v := by
-      apply SKI.s_eval_le ρ (abs e₁) (abs e₂) (.const a)
-      exact v_eval
-    have ⟨ v₁ , v₁_eval ⟩ := PAS.ap_left_defined ⟨ v , ap_abs_eval ⟩
-    have ⟨ v₂ , v₂_eval ⟩ := PAS.ap_right_defined ⟨ v , ap_abs_eval ⟩
-    apply PAS.ap_eval_ge (ρ₂ := ρ) (abs_refines_le ρ a e₁ v₁ v₁_eval) (abs_refines_le ρ a e₂ v₂ v₂_eval)
-    apply PAS.ap_eval_le v₁_eval v₂_eval
-    exact ap_abs_eval
-
-def abs_refines_ge [SKI α] (ρ : Bwd α) (a : α) (e : FreeMagma α) : (ρ :# a) ⊢ e ≤ ρ ⊢ $(abs e) a := by
-  intros v v_eval
-  match e with
-  | .var 0 =>
-    simp at *
-    have var_eval : (ρ :# a) ⊢ `(0) ⇓ a := PAS.var_zero_eval ρ a
-    apply i_eval_ge _ _
-    rw [PAS.eval_functional v_eval var_eval]
-    apply PAS.const_eval
-  | .var (n+1) =>
-    simp at *
-    apply k_eval_ge ρ (.var n) (.const a) _
-    · apply PAS.var_succ_eval_le ρ a n
-      exact v_eval
-    · apply PAS.const_defined
-  | .const b =>
-    simp at *
-    apply k_eval_ge ρ (.const b) (.const a) _
-    · apply PAS.const_eval_stable
-      exact v_eval
-    · apply PAS.const_defined
-  | .ap e₁ e₂ =>
-    simp at *
-    have ⟨ v₁ , v₁_eval ⟩ := PAS.ap_left_defined ⟨ v , v_eval ⟩
-    have ⟨ v₂ , v₂_eval ⟩ := PAS.ap_right_defined ⟨ v , v_eval ⟩
-    apply s_eval_ge ρ (abs e₁) (abs e₂) (.const a)
-    apply PAS.ap_eval_ge (ρ₂ := ρ) (abs_refines_ge ρ a e₁ v₁ v₁_eval) (abs_refines_ge ρ a e₂ v₂ v₂_eval)
-    apply PAS.ap_eval_le v₁_eval v₂_eval
-    exact v_eval
-
-end SKI
