Rz/Syntax/HOL.lean
@@ -1,0 +1,67 @@
+import Rz.Syntax.Subst
+import Rz.Data.Bwd
+
+inductive Tp : Type where
+| prod : Tp → Tp → Tp
+| fn : Tp → Tp → Tp
+| prop : Tp
+
+inductive Tm : Type where
+| var : Nat → Tm
+| pair : Tm → Tm → Tm
+| fst : Tm → Tm
+| snd : Tm → Tm
+| lam : Tm → Tm
+| app : Tm → Tm → Tm
+| and : Tm → Tm → Tm
+| or : Tm → Tm → Tm
+| implies : Tm → Tm → Tm
+| true : Tm
+| false : Tm
+| all : Tp → Tm → Tm
+| some : Tp → Tm → Tm
+| eq : Tp → Tm → Tm → Tm
+
+namespace Tm
+
+def subst (e : Tm) (σ : Sb Tm) : Tm :=
+  sorry
+-- match tm with
+-- | var => _
+-- | pair e₁ e₂ => _
+-- | fst e => _
+-- | snd : Tm → Tm
+-- | lam : Tm → Tm
+-- | app : Tm → Tm → Tm
+-- | and : Tm → Tm → Tm
+-- | or : Tm → Tm → Tm
+-- | implies : Tm → Tm → Tm
+-- | true : Tm
+-- | false : Tm
+-- | all : Tp → Tm → Tm
+-- | some : Tp → Tm → Tm
+-- | eq : Tp → Tm → Tm → Tm
+
+end Tm
+
+instance : Var Tm where
+  var := Tm.var
+
+-- TODO: Ford this :(
+inductive Entails : Bwd Tp → Bwd Tm → Tm → Type where
+| and.intro     : {Γ : Bwd Tp} → {φ : Bwd Tm} → {p q : Tm} → Entails Γ φ p → Entails Γ φ q → Entails Γ φ (Tm.and p q)
+| and.eliml     : {Γ : Bwd Tp} → {φ : Bwd Tm} → {p q : Tm} → Entails Γ φ (Tm.and p q) → Entails Γ φ p
+| and.elimr     : {Γ : Bwd Tp} → {φ : Bwd Tm} → {p q : Tm} → Entails Γ φ (Tm.and p q) → Entails Γ φ q
+| or.introl     : {Γ : Bwd Tp} → {φ : Bwd Tm} → {p q : Tm} → Entails Γ φ p → Entails Γ φ (Tm.or p q)
+| or.intror     : {Γ : Bwd Tp} → {φ : Bwd Tm} → {p q : Tm} → Entails Γ φ q → Entails Γ φ (Tm.or p q)
+| or.elim       : {Γ : Bwd Tp} → {φ : Bwd Tm} → {p q r : Tm} → Entails Γ φ (Tm.or p q) → Entails Γ (φ :# p) r → Entails Γ (φ :# q) r → Entails Γ φ r
+| implies.intro : {Γ : Bwd Tp} → {φ : Bwd Tm} → {p q : Tm} → Entails Γ (φ :# p) q → Entails Γ φ (Tm.implies p q)
+| implies.elim  : {Γ : Bwd Tp} → {φ : Bwd Tm} → {p q : Tm} → Entails Γ φ (Tm.implies p q) → Entails Γ φ p → Entails Γ φ q
+| true.intro    : {Γ : Bwd Tp} → {φ : Bwd Tm} → Entails Γ φ Tm.true
+| false.elim    : {Γ : Bwd Tp} → {φ : Bwd Tm} → {p : Tm} → Entails Γ φ Tm.false → Entails Γ φ p
+| all.intro     : {Γ : Bwd Tp} → {φ : Bwd Tm} → {A : Tp} → {p : Tm} → Entails (Γ :# A) φ p → Entails Γ φ (Tm.all A p)
+| all.elim      : {Γ : Bwd Tp} → {φ : Bwd Tm} → {A : Tp} → {p : Tm} → Entails Γ φ (Tm.all A p) → (a : Tm) → Entails Γ φ (p.subst (Sb.id ;; a))
+| some.intro    : {Γ : Bwd Tp} → {φ : Bwd Tm} → {A : Tp} → {p : Tm} → (a : Tm) → Entails Γ φ (p.subst (Sb.id ;; a)) → Entails Γ φ (Tm.some A p)
+| some.elim     : {Γ : Bwd Tp} → {φ : Bwd Tm} → {A : Tp} → {p : Tm} → Entails Γ φ (Tm.some A p) → Entails (Γ :# A) φ p
+| eq.intro      : {Γ : Bwd Tp} → {φ : Bwd Tm} → (A : Tp) → (a : Tm) → Entails Γ φ (Tm.eq A a a)
+| eq.elim       : {Γ : Bwd Tp} → {φ : Bwd Tm} → {A : Tp} → {a b : Tm} → {p : Tm} → Entails Γ φ (Tm.eq A a b) → Entails Γ φ (p.subst (Sb.id ;; a)) → Entails Γ φ (p.subst (Sb.id ;; b))
